# baseURI: http://data.sedgemoor.gov.uk/def/project/
# imports: http://data.sedgemoor.gov.uk/def/community/
# imports: http://data.sedgemoor.gov.uk/def/impact/
# imports: http://data.sedgemoor.gov.uk/def/item/
# imports: http://www.w3.org/2007/05/powder-s
# imports: http://xmlns.com/foaf/0.1/

# c14n-version: 3
@prefix owl: <http://www.w3.org/2002/07/owl#> .
@prefix project: <http://data.sedgemoor.gov.uk/def/project/> .
@prefix rdf: <http://www.w3.org/1999/02/22-rdf-syntax-ns#> .
@prefix rdfs: <http://www.w3.org/2000/01/rdf-schema#> .
@prefix skos: <http://www.w3.org/2004/02/skos/core#> .
@prefix wdrs: <http://www.w3.org/2007/05/powder-s#> .
@prefix xsd: <http://www.w3.org/2001/XMLSchema#> .
project:
  rdf:type owl:Ontology ;
  rdfs:comment "An ontology module for describing projects."@en ;
  rdfs:label "project ontology"@en ;
  owl:imports <http://data.sedgemoor.gov.uk/def/community/> ;
  owl:imports <http://data.sedgemoor.gov.uk/def/impact/> ;
  owl:imports <http://data.sedgemoor.gov.uk/def/item/> ;
  owl:imports <http://www.w3.org/2007/05/powder-s> ;
  owl:imports <http://xmlns.com/foaf/0.1/> ;
.
project:DateOrDateTime
  rdf:type rdfs:Datatype ;
  rdfs:comment ""@en ;
  rdfs:label "Date or date time"@en ;
  owl:unionOf (
      xsd:date
      xsd:dateTime
    ) ;
.
project:Project
  rdf:type owl:Class ;
  rdfs:comment "The class of projects.  This is a very general class intended to capture a very broad range of things that might be classed as projects from school homework assignments to major construction projects.  Projects usually have one or more goals.  Projects are of finite duration."@en ;
  rdfs:label "Project"@en ;
  rdfs:subClassOf owl:Thing ;
  rdfs:subClassOf [
      rdf:type owl:Restriction ;
      owl:cardinality "1"^^xsd:nonNegativeInteger ;
      owl:onProperty project:actualEnd ;
    ] ;
  rdfs:subClassOf [
      rdf:type owl:Restriction ;
      owl:cardinality "1"^^xsd:nonNegativeInteger ;
      owl:onProperty project:actualStart ;
    ] ;
  rdfs:subClassOf [
      rdf:type owl:Restriction ;
      owl:cardinality "1"^^xsd:nonNegativeInteger ;
      owl:onProperty project:expectedEnd ;
    ] ;
  rdfs:subClassOf [
      rdf:type owl:Restriction ;
      owl:cardinality "1"^^xsd:nonNegativeInteger ;
      owl:onProperty project:expectedStart ;
    ] ;
  rdfs:subClassOf [
      rdf:type owl:Restriction ;
      owl:minCardinality "0"^^xsd:nonNegativeInteger ;
      owl:onProperty <http://data.sedgemoor.gov.uk/def/impact/mitigates> ;
    ] ;
  rdfs:subClassOf [
      rdf:type owl:Restriction ;
      owl:minCardinality "0"^^xsd:nonNegativeInteger ;
      owl:onProperty project:operatesOn ;
    ] ;
  rdfs:subClassOf [
      rdf:type owl:Restriction ;
      owl:minCardinality "0"^^xsd:nonNegativeInteger ;
      owl:onProperty project:proposal ;
    ] ;
  rdfs:subClassOf [
      rdf:type owl:Restriction ;
      owl:minCardinality "0"^^xsd:nonNegativeInteger ;
      owl:onProperty project:resourcedBy ;
    ] ;
  rdfs:subClassOf [
      rdf:type owl:Restriction ;
      owl:minCardinality "0"^^xsd:nonNegativeInteger ;
      owl:onProperty project:resources ;
    ] ;
  rdfs:subClassOf [
      rdf:type owl:Restriction ;
      owl:minCardinality "0"^^xsd:nonNegativeInteger ;
      owl:onProperty <http://purl.org/dc/terms/description> ;
    ] ;
  rdfs:subClassOf [
      rdf:type owl:Restriction ;
      owl:minCardinality "0"^^xsd:nonNegativeInteger ;
      owl:onProperty rdfs:label ;
    ] ;
  rdfs:subClassOf [
      rdf:type owl:Restriction ;
      owl:minCardinality "0"^^xsd:nonNegativeInteger ;
      owl:onProperty wdrs:describedby ;
    ] ;
  owl:equivalentClass <http://xmlns.com/foaf/0.1/Project> ;
.
project:Proposal
  rdf:type owl:Class ;
  rdfs:comment "The class of proposals. A distinction is made between a proposal and a document or set of documents that describe the proposal.   Instances of the class :Proposal correspond to the action of making or submitting a proposal.  The wdrs:describedby property may be used to relate a proposal to one or more documents that describe the proposal that is made. The property community:community may be used to relate a proposal to a community to which the proposal is relevant."@en ;
  rdfs:label "Proposal"@en ;
  rdfs:subClassOf owl:Thing ;
  rdfs:subClassOf [
      rdf:type owl:Restriction ;
      owl:cardinality "1"^^xsd:nonNegativeInteger ;
      owl:onProperty project:proposalStatus ;
    ] ;
  rdfs:subClassOf [
      rdf:type owl:Restriction ;
      owl:minCardinality "0"^^xsd:nonNegativeInteger ;
      owl:onProperty <http://data.sedgemoor.gov.uk/def/community/community> ;
    ] ;
  rdfs:subClassOf [
      rdf:type owl:Restriction ;
      owl:minCardinality "0"^^xsd:nonNegativeInteger ;
      owl:onProperty <http://data.sedgemoor.gov.uk/def/impact/mitigates> ;
    ] ;
  rdfs:subClassOf [
      rdf:type owl:Restriction ;
      owl:minCardinality "0"^^xsd:nonNegativeInteger ;
      owl:onProperty project:proposedBy ;
    ] ;
  rdfs:subClassOf [
      rdf:type owl:Restriction ;
      owl:minCardinality "0"^^xsd:nonNegativeInteger ;
      owl:onProperty project:requestsResourcesFrom ;
    ] ;
  rdfs:subClassOf [
      rdf:type owl:Restriction ;
      owl:minCardinality "0"^^xsd:nonNegativeInteger ;
      owl:onProperty <http://purl.org/dc/terms/description> ;
    ] ;
  rdfs:subClassOf [
      rdf:type owl:Restriction ;
      owl:minCardinality "0"^^xsd:nonNegativeInteger ;
      owl:onProperty rdfs:label ;
    ] ;
  rdfs:subClassOf [
      rdf:type owl:Restriction ;
      owl:minCardinality "0"^^xsd:nonNegativeInteger ;
      owl:onProperty wdrs:describedby ;
    ] ;
  rdfs:subClassOf [
      rdf:type owl:Restriction ;
      owl:minCardinality "1"^^xsd:nonNegativeInteger ;
      owl:onProperty project:proposedTo ;
    ] ;
.
project:ProposalStatus
  rdf:type owl:Class ;
  rdfs:comment "The class of status's of a proposal."@en ;
  rdfs:label "Proposal status"@en ;
  rdfs:subClassOf skos:Concept ;
.
project:ResourceSource
  rdf:type owl:Class ;
  rdfs:comment "The class of resource sources."@en ;
  rdfs:label "Resource source"@en ;
  rdfs:subClassOf owl:Thing ;
  rdfs:subClassOf [
      rdf:type owl:Restriction ;
      owl:minCardinality "0"^^xsd:nonNegativeInteger ;
      owl:onProperty project:hasResourceRequest ;
    ] ;
  rdfs:subClassOf [
      rdf:type owl:Restriction ;
      owl:minCardinality "0"^^xsd:nonNegativeInteger ;
      owl:onProperty project:resources ;
    ] ;
  rdfs:subClassOf [
      rdf:type owl:Restriction ;
      owl:minCardinality "0"^^xsd:nonNegativeInteger ;
      owl:onProperty <http://purl.org/dc/terms/hasPart> ;
    ] ;
  rdfs:subClassOf [
      rdf:type owl:Restriction ;
      owl:minCardinality "0"^^xsd:nonNegativeInteger ;
      owl:onProperty <http://purl.org/dc/terms/isPartOf> ;
    ] ;
.
project:actualEnd
  rdf:type owl:DatatypeProperty ;
  rdfs:comment "The actual end time of a project."@en ;
  rdfs:domain project:Project ;
  rdfs:label "actual end"@en ;
  rdfs:range project:DateOrDateTime ;
.
project:actualStart
  rdf:type owl:DatatypeProperty ;
  rdfs:comment "The actual start time of a project."@en ;
  rdfs:domain project:Project ;
  rdfs:label "actual start"@en ;
  rdfs:range project:DateOrDateTime ;
.
project:expectedEnd
  rdf:type owl:DatatypeProperty ;
  rdfs:comment "The expected end time of a project."@en ;
  rdfs:domain project:Project ;
  rdfs:label "expected end"@en ;
  rdfs:range project:DateOrDateTime ;
.
project:expectedStart
  rdf:type owl:DatatypeProperty ;
  rdfs:comment "The expected start time of a project."@en ;
  rdfs:domain project:Project ;
  rdfs:label "expected start"@en ;
  rdfs:range project:DateOrDateTime ;
.
project:hasResourceRequest
  rdf:type owl:ObjectProperty ;
  rdfs:comment "The property :hasResourceRequest relates a resource source to a request for resource from that source."@en ;
  rdfs:domain project:ResourceSource ;
  rdfs:label "has resource request"@en ;
  rdfs:range rdfs:Resource ;
  owl:inverseOf project:requestsResourcesFrom ;
.
project:hasSubProject
  rdf:type owl:ObjectProperty ;
  rdfs:comment "Project may have subprojects.  The property :hasSubProject relates a parent project to an immediate child project."@en ;
  rdfs:domain project:Project ;
  rdfs:label "has sub project"@en ;
  rdfs:range project:Project ;
  owl:inverseOf project:isSubProjectOf ;
.
project:isSubProjectOf
  rdf:type owl:ObjectProperty ;
  rdfs:comment "Project may have subprojects.  The property :isSubProjectOf relates a project to its immediate parent project."@en ;
  rdfs:domain project:Project ;
  rdfs:label "sub project of"@en ;
  rdfs:range project:Project ;
.
project:operatesOn
  rdf:type owl:ObjectProperty ;
  rdfs:comment "The property :operatesOn relates a project to the objects that the project is intended to create or change.   For example, a project that builds a bypass operates on the bypass; a project to build a children's play area in a park could be said to operate on either the park, or the playpen or both.  A project to widen a road operates on that road."@en ;
  rdfs:domain project:Project ;
  rdfs:label "operates on"@en ;
  rdfs:range <http://data.sedgemoor.gov.uk/def/item/Item> ;
.
project:proposal
  rdf:type owl:ObjectProperty ;
  rdfs:comment "The property :hasProposal is a general purpose property that relates a resource to a proposal that is in some way related to that resource.   It can be used to relate a resource such as a project to the proposal for the creation of that resource."@en ;
  rdfs:domain rdfs:Resource ;
  rdfs:label "proposal"@en ;
  rdfs:range project:Proposal ;
.
project:proposal-status
  rdf:type skos:ConceptScheme ;
  rdfs:comment "A controlled vocabulary of proposal status values."@en ;
  rdfs:label "proposal status scheme"@en ;
  skos:hasTopConcept <http://data.sedgemoor.gov.uk/def/project/proposal-status/accepted> ;
  skos:hasTopConcept <http://data.sedgemoor.gov.uk/def/project/proposal-status/rejected> ;
.
<http://data.sedgemoor.gov.uk/def/project/proposal-status/accepted>
  rdf:type project:ProposalStatus ;
  rdfs:comment "The status of being accepted."@en ;
  rdfs:label "Status accepted"@en ;
  skos:topConceptOf project:proposal-status ;
.
<http://data.sedgemoor.gov.uk/def/project/proposal-status/rejected>
  rdf:type project:ProposalStatus ;
  rdfs:comment "The status of being rejected."@en ;
  rdfs:label "rejected"@en ;
  skos:topConceptOf project:proposal-status ;
.
project:proposalDate
  rdf:type owl:DatatypeProperty ;
  rdfs:comment "The property :proposalDate relates a proposal to the date on which the proposal was made or submitted."@en ;
  rdfs:domain project:Proposal ;
  rdfs:label "proposal date"@en ;
  rdfs:range project:DateOrDateTime ;
.
project:proposalStatus
  rdf:type owl:ObjectProperty ;
  rdfs:comment "The property :proposalStatus is a general purpose property that relates a proposal to its status."@en ;
  rdfs:domain project:Proposal ;
  rdfs:label "proposal status"@en ;
  rdfs:range project:ProposalStatus ;
.
project:proposedBy
  rdf:type owl:ObjectProperty ;
  rdfs:comment "The property :proposedBy is a general purpose property that relates a proposal to a an agent making the proposal."@en ;
  rdfs:domain project:Proposal ;
  rdfs:label "proposed by"@en ;
  rdfs:range <http://xmlns.com/foaf/0.1/Agent> ;
.
project:proposedTo
  rdf:type owl:ObjectProperty ;
  rdfs:comment "The property :proposedBy relates a proposal to an agent to whom the proposal is made."@en ;
  rdfs:domain project:Proposal ;
  rdfs:label "proposed to"@en ;
  rdfs:range <http://xmlns.com/foaf/0.1/Agent> ;
.
project:requestsResourcesFrom
  rdf:type owl:ObjectProperty ;
  rdfs:comment "The property :requestsResourcesFrom is a general purpose property that relates a resource such as a proposal to a source of resources from which resources are requested."@en ;
  rdfs:domain rdfs:Resource ;
  rdfs:label "requires resources from"@en ;
  rdfs:range project:ResourceSource ;
  owl:inverseOf project:hasResourceRequest ;
.
project:resourcedBy
  rdf:type owl:ObjectProperty ;
  rdfs:comment "The property :resourcedBy is a general purpose property that relates a consumer of resource such as a project to a source of resource such as a Fund"@en ;
  rdfs:domain rdfs:Resource ;
  rdfs:label "resources"@en ;
  rdfs:range project:ResourceSource ;
  owl:inverseOf project:resources ;
.
project:resources
  rdf:type owl:ObjectProperty ;
  rdfs:comment "The property :resources is a general purpose property that relates a source of resource to a consumer of resources such as a project."@en ;
  rdfs:domain rdfs:Resource ;
  rdfs:label "resources"@en ;
  rdfs:range rdfs:Resource ;
  owl:inverseOf project:resourcedBy ;
.
