# baseURI: http://data.sedgemoor.gov.uk/def/version/
# imports: http://purl.org/dc/terms/

# c14n-version: 3
@prefix owl: <http://www.w3.org/2002/07/owl#> .
@prefix rdf: <http://www.w3.org/1999/02/22-rdf-syntax-ns#> .
@prefix rdfs: <http://www.w3.org/2000/01/rdf-schema#> .
@prefix version: <http://data.sedgemoor.gov.uk/def/version/> .
@prefix xsd: <http://www.w3.org/2001/XMLSchema#> .
version:
  rdf:type owl:Ontology ;
  rdfs:comment "A small ontology with some basic terms for representing versions."@en ;
  rdfs:label "Version Ontology"@en ;
  owl:imports <http://purl.org/dc/terms/> ;
.
version:Version
  rdf:type owl:Class ;
  rdfs:comment "The class of versions.  A version is a version of a versioned thing."@en ;
  rdfs:label "Version"@en ;
  rdfs:subClassOf owl:Thing ;
  rdfs:subClassOf [
      rdf:type owl:Restriction ;
      owl:cardinality "1"^^xsd:nonNegativeInteger ;
      owl:onProperty version:identifier ;
    ] ;
  rdfs:subClassOf [
      rdf:type owl:Restriction ;
      owl:maxCardinality "1"^^xsd:nonNegativeInteger ;
      owl:onProperty version:date ;
    ] ;
  rdfs:subClassOf [
      rdf:type owl:Restriction ;
      owl:onClass version:VersionedThing ;
      owl:onProperty <http://purl.org/dc/terms/isVersionOf> ;
      owl:qualifiedCardinality "1"^^xsd:nonNegativeInteger ;
    ] ;
.
version:VersionedThing
  rdf:type owl:Class ;
  rdfs:comment "The class of versioned things.  A versioned thing is a thing which may have more than one version."@en ;
  rdfs:label "Versioned thing"@en ;
  rdfs:subClassOf owl:Thing ;
  rdfs:subClassOf [
      rdf:type owl:Restriction ;
      owl:minQualifiedCardinality "0"^^xsd:nonNegativeInteger ;
      owl:onClass version:Version ;
      owl:onProperty <http://purl.org/dc/terms/hasVersion> ;
    ] ;
.
version:date
  rdf:type owl:DatatypeProperty ;
  rdfs:comment "The :dateProperty relates a version to 'the date' of that version.  What constitutes 'the date' of a version depends on the type of thing that is being versioned.  For example, the :date of a version of a publication might be the date that particular version was finalized.."@en ;
  rdfs:domain version:Version ;
  rdfs:label "date"@en ;
  rdfs:range xsd:date ;
.
version:identifier
  rdf:type owl:DatatypeProperty ;
  rdfs:comment "The property :identifier relates a version to an identifier uniquely identifying that version  of the versioned thing."@en ;
  rdfs:domain version:Version ;
  rdfs:label "version identifier"@en ;
  rdfs:range xsd:string ;
.
